Hack to avoid typeclasses

io/ModelingLanguage.fst
@@ -25,15 +25,19 @@ let pi_type = monitorable_prop
 noeq
 type interface = {
   pi : pi_type;
+  ictx_in : Type u#a;
+  ictx_out : Type u#b;
+  iprog_out : Type u#c; 
+
   ctx_in : Type u#a;
   ctx_out : Type u#b;
   prog_out : Type u#c; 
 }
 
 (** *** Intermediate Lang **)
-type ictx (i:interface) = x:i.ctx_in -> ILang.IIOpi i.ctx_out i.pi
-type iprog (i:interface) = ictx i -> ILang.IIOpi i.prog_out i.pi
-type iwhole (i:interface) = unit -> ILang.IIOpi i.prog_out i.pi
+type ictx (i:interface) = x:i.ictx_in -> ILang.IIOpi i.ictx_out i.pi
+type iprog (i:interface) = ictx i -> ILang.IIOpi i.iprog_out i.pi
+type iwhole (i:interface) = unit -> ILang.IIOpi i.iprog_out i.pi
 let ilink (i:interface) (ip:iprog i) (ic:ictx i) : iwhole i = fun () -> ip ic
 
 (** *** Target Lang **)
@@ -49,24 +53,36 @@ type prog (i:interface) = ctx i -> pt i free
 type whole (i:interface) (mon:monad) = unit -> pt i mon
 let link (i:interface) (p:prog i) (c:ctx i) : whole i free = fun () -> p c
 
+(* TODO: to avoid to do typeclasses *)
+assume val backtranslate' : (i:interface) -> i.ctx_out -> i.ictx_out
+assume val compile' : (i:interface) -> i.ictx_in -> i.ctx_in
+assume val compile'' : (i:interface) -> i.iprog_out -> i.prog_out
+
 (** *** Backtranslate **)
 (* TODO: these will need to be type-classes depending on structure of ct and pt *)
 val backtranslate : (i:interface) -> ctx i -> acts free -> ictx i
-let backtranslate i c (ca:acts free) (x:i.ctx_in) : ILang.IIOpi i.ctx_out i.pi =
+let backtranslate i c (ca:acts free) (x:i.ictx_in) : ILang.IIOpi i.ictx_out i.pi =
   let c : ct i free = c free ca in
-  let tree : iio i.ctx_out = c x in
+  let tree : iio i.ctx_out = c (compile' i x) in
   assume (tree `has_type` dm_iio i.ctx_out (ILang.pi_hist i.ctx_out i.pi)); 
   let dm_tree : dm_iio i.ctx_out (ILang.pi_hist i.ctx_out i.pi) = tree in
-  IIOwp?.reflect dm_tree
+  let r : i.ctx_out = IIOwp?.reflect dm_tree in
+  backtranslate' i r
+
+(* Case 1: We want to backtranslate a first order context. It should be rather simple to 
+do that **)
+
+(* Case 2: We want to backtranslate a higher order context. **)
+
 
 (** *** Compilation **)
 (* TODO: this needs to be/include IIO pi arrow; which may bring back reification? in compile_whole? on the argument of compile_whole? *)
 (* CA: What does reify do if `ip` is returning an arrow? **)
 let compile (i:interface) (ip:iprog i) (ca:acts free) : prog i = 
   fun (c:ctx i) -> 
-    let tree : dm_iio i.prog_out (ILang.pi_hist _ i.pi) = 
+    let tree : dm_iio i.iprog_out (ILang.pi_hist _ i.pi) = 
       reify (ip (backtranslate i c ca)) in
-    tree
+    iio_bind tree (fun x -> Return (compile'' i x))
 
 
 (* now we can better write backtranslate; TODO: but to typecheck it we need parametricity? *)
